theories/GeneralizeLtsOutputs.v
@@ -34,7 +34,7 @@ Require Import Coq.Program.Equality.
 From Coq.Logic Require Import ProofIrrelevance.
 
 From stdpp Require Import base countable list decidable finite gmap gmultiset.
-From Must Require Import TransitionSystems OldTransitionSystems.
+From Must Require Import TransitionSystems OldTransitionSystems VCCS_Instance Subset_Act.
 
 (* Genarilization via essential actions, non_blocking actions *)
 
@@ -88,15 +88,36 @@ Proof.
   refine (inj_countable encode_ext_act decode_ext_act encode_decide_ext_act).
 Qed.
 
-#[global] Program Instance gLabel
-  `{Label A} : TransitionSystems.ExtAction (ExtAct A).
+Definition all_blocking_action `{Label A} (μ : ExtAct A) := False.
+
+#[global] Program Instance all_blocking_action_dec `{Label A} μ :
+    Decision (all_blocking_action μ).
 Next Obligation.
-  intros L H μ. exact (is_output μ).
+  intros. right. intro imp. inversion imp.
+Defined.
+
+Definition output_are_non_blocking `{Label A} (μ : ExtAct A) := (is_output μ).
+
+#[global] Program Instance output_are_non_blocking_dec `{Label A} μ :
+    Decision (output_are_non_blocking μ).
+Next Obligation.
+  intros. destruct μ as [a | a].
+  + right. intro imp. inversion imp; eauto. inversion H0.
+  + left. exists a. eauto.
+Defined.
+
+(* ExtAction for output are non_blocking *)
+
+#[global] Program Instance gLabel_nb
+  `{Label A} :
+        TransitionSystems.ExtAction (ExtAct A).
+Next Obligation.
+  intros L H μ. exact (output_are_non_blocking μ).
 Defined.
 Next Obligation.
- intros. destruct a.
- + right. intro imp. destruct imp as (μ & eq). subst. inversion eq.
- + left. exists a. eauto.
+ intros. simpl. destruct a.
+ * right. intro Hyp. destruct Hyp as (a' & eq). inversion eq.
+ * left. exists a. eauto.
 Defined.
 Next Obligation.
   intros A H μ1. exact (co μ1).
@@ -106,11 +127,11 @@ Next Obligation.
 Defined.
 Next Obligation.
   intros. exists (co η). unfold sc. 
-  unfold gLabel_obligation_4. unfold ext_act_match.
+  unfold gLabel_nb_obligation_4. unfold ext_act_match.
   destruct η; simpl in *; eauto. 
 Defined.
 Next Obligation.
-  intros. unfold sc. unfold gLabel_obligation_4.
+  intros. unfold sc. unfold gLabel_nb_obligation_4.
   destruct a; destruct b.
   + right. intro cases. eauto. destruct cases as [case_1 | case_2].
     ++ eapply simplify_match_input in case_1. inversion case_1.
@@ -130,8 +151,8 @@ Next Obligation.
   + simpl in *. right. intro Hyp. destruct Hyp; eauto.
 Defined.
 Next Obligation.
-  unfold gLabel_obligation_1.
-  unfold gLabel_obligation_4.
+  unfold gLabel_nb_obligation_4.
+  unfold gLabel_nb_obligation_1.
   intros A H η μ IsOut eq.
   intro IsOut'. destruct IsOut' as (μ' & eq'); subst.
   unfold sc in eq.
@@ -145,9 +166,9 @@ Next Obligation.
     inversion impossible.
 Defined.
 Next Obligation.
-  unfold gLabel_obligation_1.
-  unfold gLabel_obligation_4.
-  unfold sc. unfold gLabel_obligation_3.
+  unfold gLabel_nb_obligation_1.
+  unfold gLabel_nb_obligation_4.
+  unfold sc. unfold gLabel_nb_obligation_3.
   intros A H η μ IsOut eq.
   destruct IsOut as (η' & eq'); subst.
   destruct eq as [eq_1 | eq_2].
@@ -156,8 +177,8 @@ Next Obligation.
     eapply simplify_match_output in eq_2. subst. simpl. eauto.
 Defined.
 Next Obligation. 
-  unfold sc. unfold gLabel_obligation_1.
-  unfold gLabel_obligation_4.
+  unfold sc. unfold gLabel_nb_obligation_1.
+  unfold gLabel_nb_obligation_4.
   intros A ? ? ? ? (a & eq) Hyp Hyp'. subst.
   destruct Hyp as [case_1 | case_2]; destruct Hyp' as [case_1' | case_2']; exists a; eauto.
   + eapply simplify_match_output in case_1. subst.
@@ -172,74 +193,106 @@ Next Obligation.
     eapply simplify_match_output in case_2. subst.
     eapply simplify_match_input in case_2'. subst.
     eauto.
+Qed.
+
+#[global] Program Instance gLabel_b
+  `{Label A} :
+        TransitionSystems.ExtAction (ExtAct A).
+Next Obligation.
+  intros L H μ. exact (all_blocking_action μ).
+Defined.
+Next Obligation.
+ intros. simpl. exact False_dec.
+Defined.
+Next Obligation.
+  intros.
+  simpl in *. intros. inversion H0.
+  (* intros A H μ1. exact (co μ1). *)
+Defined.
+Next Obligation.
+  intros A H μ1. exact (co μ1).
+Defined.
+Next Obligation.
+  simpl in *.
+  intros. inversion H0. (* unfold relation. exact ext_act_match. *)
+Defined.
+Next Obligation.
+  intros. exists (co η). unfold sc. unfold parallel_inter. unfold dual. simpl. 
+  unfold gLabel_nb_obligation_4. left. unfold ext_act_match.
+  destruct η; simpl in *; eauto. 
+Defined.
+Next Obligation.
+  intros. unfold sc. unfold gLabel_nb_obligation_4.
+  simpl in *. inversion H0.
 Defined.
 
 
-#[global] Program Instance gLts
-  `{LtsP: Lts P A} : gLts P (ExtAct A).
+#[global] Program Instance ggLts {A : Type}
+  (H : ExtAction (ExtAct A)) `{LtsP: Lts P A} : @gLts P (ExtAct A) H.
 Next Obligation.
-  intros ? ? ? ? p1 α p2.
+  intros ? ? ? ? ? p1 α p2.
   destruct α as [|].
   + exact (lts_step p1 (ActExt μ) p2).
   + exact (lts_step p1 τ p2).
 Defined.
 Next Obligation.
-  intros ? ? ? ? p1 α p2. unfold gLts_obligation_1.
+  intros ? ? ? ? ? p1 α p2. unfold ggLts_obligation_1.
   destruct α as [ μ |].
   + exact (lts_step_decidable p1 (ActExt μ) p2).
   + exact (lts_step_decidable p1 τ p2).
 Defined.
 Next Obligation.
-  intros ? ? ? LtsP p α. 
+  intros ? ? ? ? LtsP p α. 
   destruct α as [ μ |].
   + exact (lts_stable p (ActExt μ)).
   + exact (lts_stable p τ).
 Defined.
 Next Obligation.
-  unfold gLts_obligation_3.
+  unfold ggLts_obligation_3.
   destruct α as [ μ |].
   + exact (lts_stable_decidable p (ActExt μ)).
   + exact (lts_stable_decidable p τ).
 Defined.
 Next Obligation.
-  unfold gLts_obligation_3.
+  unfold ggLts_obligation_3.
   destruct α as [ μ |].
   + intro not_stable. exact (lts_stable_spec1 p (ActExt μ) not_stable).
   + intro not_stable. exact (lts_stable_spec1 p τ not_stable).
 Qed.
 Next Obligation.
-  unfold gLts_obligation_1.
-  unfold gLts_obligation_3.
+  unfold ggLts_obligation_1.
+  unfold ggLts_obligation_3.
   destruct α as [ μ |].
   + intro wit_not_stable. exact (lts_stable_spec2 p (ActExt μ) wit_not_stable).
   + intro wit_not_stable. exact (lts_stable_spec2 p τ wit_not_stable).
-Defined.
+Qed.
 
 
-#[global] Program Instance gFiniteLts
-  `{FiniteLts P A} : FiniteImagegLts P (ExtAct A).
+#[global] Program Instance ggFiniteLts {A : Type}
+  (H : ExtAction (ExtAct A)) `{FiniteLts P A} : @FiniteImagegLts P (ExtAct A) H (ggLts H).
 Next Obligation.
   intros.
   destruct α as [ μ |].
   + exact (folts_next_states_finite p (ActExt μ)).
   + exact (folts_next_states_finite p τ).
-Defined.
+Qed.
 
-#[global] Program Instance gLtsEq
-  `{LtsEq P A} : gLtsEq P (ExtAct A).
+#[global] Program Instance ggLtsEq {A : Type}
+  (H : ExtAction (ExtAct A)) `{LtsEq P A} : @gLtsEq P (ExtAct A) H (ggLts H).
 Next Obligation.
-  intros ? ? ? LtsP LtsEqP p q α Hyp. 
+  intros ? ? ? ? LtsP LtsEqP p q α Hyp.
   destruct α as [ μ |].
   + exact (eq_spec p q (ActExt μ) Hyp).
   + exact (eq_spec p q τ Hyp).
-Defined.
+Qed.
 
 Definition label_to_output `{Label A} (a : A) : ExtAct A := ActOut a.
 
 Definition mo_label_to_mo_output `{Label A} (m : gmultiset A) : gmultiset (ExtAct A) :=
     gmultiset_map label_to_output m.
 
-Definition set_label_to_mo_output `{Label A} (m : gset A) : gset (ExtAct A) :=
+Definition set_label_to_mo_output `{Label A}
+    (m : gset A) : gset (ExtAct A) :=
     list_to_set (fmap label_to_output (elements m)).
 
 (* #[global] Instance output_in_gmultiset_dec `{Prop_of_Inter S1 S2 A} 
@@ -247,14 +300,14 @@ Definition set_label_to_mo_output `{Label A} (m : gset A) : gset (ExtAct A) :=
   Decision (η = label_to_output x ∧ x ∈ lts_oba_mo p1). *)
 
 
-#[global] Program Instance gLtsOba
-  `{LtsOba P A} : gLtsOba P (ExtAct A).
+#[global] Program Instance ggLtsOba_nb
+  `{LtsOba P A} : @gLtsOba P (ExtAct A) gLabel_nb (ggLts gLabel_nb) (ggLtsEq gLabel_nb).
 Next Obligation.
   intros.
   exact (mo_label_to_mo_output (lts_oba_mo p)).
 Defined.
 Next Obligation.
-  intros ? ? ? ? ? ? ? ? ? nb l. unfold gLtsOba_obligation_1.
+  intros ? ? ? ? ? ? ? ? ? nb l.
   destruct η as [a | a].
   + exfalso. inversion nb. inversion H2.
   + eapply elem_of_gmultiset_map.
@@ -265,7 +318,6 @@ Next Obligation.
          exact l.
 Defined.
 Next Obligation.
-  unfold gLtsOba_obligation_1.
   intros ? ? ? ? ? ? ? ? Hyp. 
   eapply elem_of_gmultiset_map in Hyp.
   
@@ -284,7 +336,7 @@ Next Obligation.
     ++ rewrite eq. unfold label_to_output. exact l.
 Qed.
 Next Obligation.
-  unfold gLtsOba_obligation_1.
+  unfold ggLtsOba_nb_obligation_1.
   intros ? ? ? ? ? LtsOBAP ? ? ? nb Hyp;simpl in *.
   destruct nb as (a & eq). subst.
   assert (lts_oba_mo p = {[+ a +]} ⊎ lts_oba_mo q) as mem.
@@ -295,7 +347,7 @@ Next Obligation.
 Qed.
 Next Obligation. (* lts_oba_non_blocking_action_delay *)
   intros ? ? ? ? ? LtsOBAP ? ? ? ? ? nb l1 l2 ;simpl in *.
-  unfold gLts_obligation_1 in l2.
+  unfold ggLts_obligation_1 in l2.
   destruct nb as (a & eq); subst. 
   destruct α as [|].
   + destruct μ as [a' | a'].
@@ -311,11 +363,11 @@ Qed.
 Next Obligation. (* lts_oba_output_tau *)
   intros ? ? ? ? ? LtsOBAP ? ? ? ? nb l1 l2 ;simpl in *.
   destruct nb as (a & eq); subst.
-  unfold gLabel_obligation_4.
+  unfold gLabel_nb_obligation_4.
   eapply lts_oba_output_tau in l1 as cases; eauto.
   destruct cases as [computation_without_a | computation_with_a].
-  + left. destruct computation_without_a as (t & l'1 & l'2).
-    exists t; eauto.
+  + left. destruct computation_without_a. 
+    eexists; eauto.
   + right. exists (ActIn a). split; eauto.
     unfold sc. simpl. eauto.
 Qed.
@@ -330,8 +382,9 @@ Next Obligation. (* lts_oba_non_blocking_action_deter_inv *)
   eapply lts_oba_output_deter_inv; eauto.
 Qed.
 
-#[global] Program Instance gLtsObaFB
-  `{LtsObaFB P A} : gLtsObaFB P (ExtAct A).
+#[global] Program Instance ggLtsObaFB_nb
+  `{LtsObaFB P A} : @gLtsObaFB P (ExtAct A) gLabel_nb 
+  (ggLts gLabel_nb) (ggLtsEq gLabel_nb) ggLtsOba_nb.
 Next Obligation.
   intros ? ? ? ? ? LtsOBAP ? ? ? ? ? ? nb duo l1 l2 ;simpl in *.
   destruct nb as (a & eq); subst.
@@ -343,29 +396,160 @@ Next Obligation.
     eapply lts_oba_fb_feedback; eauto.
 Qed.
 
-#[global] Program Instance gLtsObaFW
-  `{LtsObaFW P A} : gLtsObaFW P (ExtAct A).
+#[global] Program Instance ggLtsObaFW_nb
+  `{LtsObaFW P A} : @gLtsObaFW P (ExtAct A) gLabel_nb 
+  (ggLts gLabel_nb) (ggLtsEq gLabel_nb) ggLtsOba_nb.
 Next Obligation.
   intros ? ? ? ? ? ? ? p η μ ;simpl in *.
-  destruct (decide (non_blocking η)) as [nb | not_nb].
+  destruct (decide (gLabel_nb_obligation_1 A H η)) as [nb | not_nb].
   + destruct nb as (a & eq); subst.
-    unfold gLabel_obligation_1. unfold gLabel_obligation_4.
+    unfold gLabel_nb_obligation_1. unfold gLabel_nb_obligation_4.
     destruct (lts_oba_fw_forward p a) as (p' & l1 & l2).
     exists p'. intros Hyp duo. destruct duo as [case_1 | case_2].
     ++ eapply simplify_match_output in case_1; subst. split;eauto.
     ++ eapply symmetry, simplify_match_output in case_2; subst. split;eauto.
   + exists p. intro. contradiction.
 Qed.
-
-#[global] Program Instance Inter_FW
-  `{LtsP : Lts P A} : 
-    Prop_of_Inter P (TransitionSystems.mb (ExtAct A)) (ExtAct A) fw_inter.
 Next Obligation.
-  intros ? ? ? ? p. exact (set_label_to_mo_output (lts_outputs p)).
+  intros ? ? ? ? ? ? ? p p' p'' η μ nb duo l1 l2;simpl in *.
+  destruct nb as (a & eq); subst.
+  destruct duo as [case_1 | case_2].
+  + eapply simplify_match_output in case_1; subst.
+    eapply lts_oba_fw_feedback in l1; eauto.
+  + symmetry in case_2. eapply simplify_match_output in case_2; subst.
+    eapply lts_oba_fw_feedback in l1; eauto.
+Qed.
+
+
+#[global] Program Instance ggLtsOba_b
+  `{LtsEqP : @LtsEq P A H LtsP} :
+    @gLtsOba P (ExtAct A) (@gLabel_b A H) 
+    (@ggLts A gLabel_b P H LtsP) (@ggLtsEq A gLabel_b P H LtsP LtsEqP).
+Next Obligation.
+  intros.
+  exact empty.
 Defined.
 Next Obligation.
-  unfold Inter_FW_obligation_1. unfold set_label_to_mo_output.
-  intros ? ? ? ? ? ? Hyp ;simpl in *.
+  intros. inversion H0.
+Defined.
+Next Obligation.
+  intros ? ? ? ? ? ? ? mem. simpl in *. exists p1. inversion mem.
+Qed.
+Next Obligation.
+  intros ? ? ? ? ? ? ? ? imp. inversion imp.
+Qed.
+Next Obligation.
+  intros ? ? ? ? ? ? ? ? ? ? Hyp. inversion Hyp.
+Qed.
+Next Obligation. (* lts_oba_non_blocking_action_delay *)
+  intros ? ? ? ? ? LtsOBAP ? ? ? ? mem. inversion mem.
+Qed.
+Next Obligation. (* lts_oba_non_blocking_action_confluence *)
+  intros ? ? ? ? ? LtsOBAP ? ? ? mem. inversion mem.
+Qed.
+Next Obligation. (* lts_oba_output_tau *)
+  intros ? ? ? ? ? LtsOBAP ? ? ? imp. inversion imp.
+Qed.
+Next Obligation. (* lts_oba_output_deter *)
+  intros ? ? ? ? ? LtsOBAP ? ? ? ? imp. inversion imp.
+Qed.
+
+#[global] Program Instance ggLtsObaFB_b
+  `{LtsEqP : @LtsEq P A H LtsP} : @gLtsObaFB P (ExtAct A) gLabel_b 
+  (ggLts gLabel_b) (ggLtsEq gLabel_b) ggLtsOba_b.
+Next Obligation.
+  intros ? ? ? ? ? LtsOBAP ? ? ? ? imp. inversion imp.
+Qed.
+
+#[global] Program Instance ggLtsObaFW_b
+  `{LtsEqP : @LtsEq P A H LtsP} : @gLtsObaFW P (ExtAct A) gLabel_b 
+  (ggLts gLabel_b) (ggLtsEq gLabel_b) ggLtsOba_b.
+Next Obligation.
+  intros ? ? ? ? ? ? ? ?. exists p1. intro imp. inversion imp.
+Qed.
+Next Obligation.
+  intros ? ? ? ? ? ? ? ? ? ? imp. inversion imp.
+Qed.
+
+
+#[global] Program Instance Inter_FW {A : Type} (H : ExtAction (ExtAct A))
+  `{LtsP : Lts P A} {ext_m : forall μ1 μ2, dual μ1 μ2 = ext_act_match μ1 μ2}: 
+    Prop_of_Inter P (TransitionSystems.mb (ExtAct A)) (ExtAct A) fw_inter.
+Next Obligation.
+  intros ? ? ? ? ? ? p. exact empty.
+Defined.
+Next Obligation. 
+  unfold Inter_FW_obligation_1. 
+  intros ? ? ? ? ? ? ? ? Hyp ;simpl in *.
+  inversion Hyp.
+Qed.
+Next Obligation.
+  intros ? ? ? ? ? ? m;simpl in *.
+  exact (dom (mb_without_not_nb m)).
+Defined.
+Next Obligation.
+  unfold Inter_FW_obligation_3.
+  intros ? ? ? ? ? ? m ? Hyp ;simpl in *.
+  eapply gmultiset_elem_of_dom in Hyp. 
+  assert (ξ ∈ mb_without_not_nb m) as mem. eauto.
+  eapply lts_mb_nb_with_nb_spec1 in mem as (nb & eq).
+  eapply gmultiset_disj_union_difference' in eq.
+  exists (m ∖ {[+ ξ +]}). rewrite eq at 1.
+  eapply lts_multiset_minus; eauto.
+Defined.
+Next Obligation.
+  intros ? ? ? ? ? ? ? ? ? m ? m' ? ? inter;simpl in *.
+  right. destruct inter as (duo & nb).
+  unfold Inter_FW_obligation_3.
+  eapply gmultiset_elem_of_dom.
+  eapply non_blocking_action_in_ms in nb as eq'; eauto. 
+  rewrite<- eq'.
+  assert (mb_without_not_nb ({[+ α2 +]} ⊎ m') 
+  = {[+ α2 +]} ⊎ (mb_without_not_nb m')) as eq.
+  eapply lts_mb_nb_spec1; eauto. rewrite eq.
+  multiset_solver.
+Defined.
+Next Obligation.
+  intros ? ? ? ? ? ? ξ p;simpl in *.
+  destruct (decide (non_blocking ξ)) as [ nb (* Input_case *) | not_nb (* Ouput_case *)].
+  + exact {[ co ξ ]}.
+  + exact empty.
+Defined.
+Next Obligation.
+  unfold Inter_FW_obligation_6.
+  unfold Inter_FW_obligation_3.
+  intros ? ? ? ? ? ? ? ? ? ? m mem l inter;simpl in *.
+  destruct inter as (duo & nb). rewrite decide_True; eauto.
+
+  assert (μ = co ξ). rewrite ext_m in duo.
+  destruct ξ as [a | a].
+  + eapply simplify_match_input in duo; subst; eauto.
+  + eapply simplify_match_output in duo; subst; eauto.
+  
+  + subst; set_solver.
+Defined.
+Next Obligation.
+  intros. exact empty.
+Defined.
+Next Obligation.
+  unfold Inter_FW_obligation_8. unfold Inter_FW_obligation_1.
+  intros ? ? ? ? ? ? ? ? ? ? m mem l inter;simpl in *.
+  inversion mem.
+Qed.
+
+(* #[global] Program Instance Inter
+  `{Lts P A} `{Lts Q A} (H : ExtAction (ExtAct A))
+    {ext_m : forall μ1 μ2, dual μ1 μ2 = ext_act_match μ1 μ2}: 
+    Prop_of_Inter P Q (ExtAct A) parallel_inter.
+Next Obligation.
+  intros ? ? ? ? ? ? ? ? p. 
+  Check (set_label_to_mo_output (lts_outputs p)). Check (@lts_outputs).
+  exact (@set_label_to_mo_output A L (lts_outputs p)). 
+Admitted.
+Next Obligation.
+  intros ? ? ? ? ? ? p ? Hyp ;simpl in *.
+  unfold Inter_FW_obligation_1 in Hyp.
+  unfold set_label_to_mo_output in Hyp.
   eapply elem_of_list_to_set in Hyp.
   eapply elem_of_list_fmap in Hyp.
 
@@ -383,35 +567,55 @@ Next Obligation.
     eapply elem_of_elements; eauto.
     eapply lts_outputs_spec2 in mem'. 
     eauto.
-Qed.
-Next Obligation.
-  intros ? ? ? ? m;simpl in *.
-  exact (dom (mb_without_not_nb m)).
 Defined.
 Next Obligation.
-  unfold Inter_FW_obligation_3.
-  intros ? ? ? ? m ? Hyp ;simpl in *.
-  eapply gmultiset_elem_of_dom in Hyp. 
-  assert (ξ ∈ mb_without_not_nb m) as mem. eauto.
-  eapply lts_mb_nb_with_nb_spec1 in mem as (nb & eq).
-  eapply gmultiset_disj_union_difference' in eq.
-  exists (m ∖ {[+ ξ +]}). rewrite eq at 1.
-  eapply lts_multiset_minus; eauto.
+  intros ? ? ? ? ? ? q;simpl in *.
+  exact (set_label_to_mo_output (lts_outputs q)).
 Defined.
 Next Obligation.
-  intros ? ? ? ? ? ? ? m ? m' ? ? inter;simpl in *.
-  right. destruct inter as (duo & nb).
-  unfold Inter_FW_obligation_3.
-  eapply gmultiset_elem_of_dom.
-  eapply non_blocking_action_in_ms in nb as eq'; eauto. 
-  rewrite<- eq'.
-  assert (mb_without_not_nb ({[+ α2 +]} ⊎ m') 
-  = {[+ α2 +]} ⊎ (mb_without_not_nb m')) as eq.
-  eapply lts_mb_nb_spec1; eauto. rewrite eq.
-  multiset_solver.
+  intros ? ? ? ? ? ? q ? Hyp ;simpl in *.
+  unfold Inter_FW_obligation_1 in Hyp.
+  unfold set_label_to_mo_output in Hyp.
+  eapply elem_of_list_to_set in Hyp.
+  eapply elem_of_list_fmap in Hyp.
+
+  assert {x : A | ξ = label_to_output x ∧ x ∈ elements (lts_outputs q)} as wit.
+  eapply choice;eauto. intro.
+  destruct (decide (ξ = label_to_output x)).
+  + destruct (decide (x ∈ elements (lts_outputs q))).
+    ++ left; eauto.
+    ++ right. intros (Hyp1 & imp). contradiction.
+  + right. intros (imp & Hyp2). contradiction.
+  
+  + destruct wit as ( a & eq & mem ).
+    unfold label_to_output in eq; subst.
+    assert (a ∈ lts_outputs q) as mem'.
+    eapply elem_of_elements; eauto.
+    eapply lts_outputs_spec2 in mem'. 
+    eauto.
 Defined.
 Next Obligation.
-  intros ? ? ? ? ξ p;simpl in *.
+  intros ? ? ? ? ? ? ? ? ? q ? q' ? ? inter;simpl in *.
+  unfold Inter_par_obligation_1. unfold Inter_par_obligation_3.
+  destruct α1 as [a (* input a *) | a (* output b *)].
+  + right. destruct inter as [case_1 | case_2].
+    ++ symmetry in case_1. eapply simplify_match_input in case_1 as eq; subst.
+       unfold set_label_to_mo_output.
+       eapply elem_of_list_to_set.
+       eapply elem_of_list_fmap. exists a. split; eauto. 
+       eapply elem_of_elements. eapply lts_outputs_spec1; eauto.
+    ++ eapply simplify_match_input in case_2 as eq; subst.
+       unfold set_label_to_mo_output.
+       eapply elem_of_list_to_set.
+       eapply elem_of_list_fmap. exists a. split; eauto. 
+       eapply elem_of_elements. eapply lts_outputs_spec1; eauto.
+  + left. 
+    eapply elem_of_list_to_set.
+    eapply elem_of_list_fmap. exists a. split; eauto. 
+    eapply elem_of_elements. eapply lts_outputs_spec1; eauto.
+Defined.
+Next Obligation.
+  intros ? ? ? ? ? ? ξ p;simpl in *.
   destruct ξ as [ a (* Input_case *) | a (* Ouput_case *)].
   + exact empty. 
   + exact {[ ActIn a ]}.
@@ -419,77 +623,235 @@ Defined.
 Next Obligation.
   unfold Inter_FW_obligation_6.
   unfold Inter_FW_obligation_3.
-  intros ? ? ? ? ? ? ? ? m mem l inter;simpl in *.
-  destruct inter as (duo & nb). destruct nb as (a & eq).
-  subst. destruct duo as [case_1 | case_2]; unfold gLabel_obligation_4 in *.
+  intros ? ? ? ? ? ? ? ? ? ? q mem l inter;simpl in *. 
+  eapply elem_of_list_to_set in mem.
+  eapply elem_of_list_fmap in mem.
+  destruct mem as ( a & eq & mem ); subst. simpl.
+  destruct inter as [case_1 | case_2]; unfold gLabel_nb_obligation_4 in *.
   + eapply simplify_match_output in case_1. subst. set_solver.
   + symmetry in case_2. eapply simplify_match_output in case_2. subst. set_solver.
 Defined.
 Next Obligation.
-  intros. exact empty.
+  intros ? ? ? ? ? ? ξ q;simpl in *.
+  destruct ξ as [ a (* Input_case *) | a (* Ouput_case *)].
+  + exact empty. 
+  + exact {[ ActIn a ]}.
 Defined.
 Next Obligation.
-  unfold Inter_FW_obligation_8. unfold Inter_FW_obligation_1.
-  intros ? ? ? ? ? ? ? ? m mem l inter;simpl in *.
-  exfalso.
-  destruct inter as (duo & nb). destruct nb as (a & eq). subst.
-  unfold set_label_to_mo_output in mem.
+  unfold Inter_FW_obligation_6.
+  unfold Inter_FW_obligation_3.
+  intros ? ? ? ? ? ? ? ? ? ? q mem l inter;simpl in *. 
   eapply elem_of_list_to_set in mem.
-  eapply elem_of_list_fmap in mem. destruct mem as (a' & eq & mem').
-  subst. destruct duo as [case_1 | case_2].
-  + eapply simplify_match_output in case_1. inversion case_1.
-  + eapply simplify_match_output in case_2. inversion case_2.
+  eapply elem_of_list_fmap in mem.
+  destruct mem as ( a & eq & mem ); subst. simpl.
+  destruct inter as [case_1 | case_2]; unfold gLabel_nb_obligation_4 in *.
+  + symmetry in case_1. eapply simplify_match_output in case_1. subst. set_solver.
+  + eapply simplify_match_output in case_2. subst. set_solver.
+Defined. *)
+
+(* #[global] Program Instance Inter_FW_par_nb
+  `{@Lts P A H} `{@Lts E A H}
+  : Prop_of_Inter (P * mb A) E (ExtAct A) parallel_inter.
+Next Obligation.
+  intros ? ? ? ? ? ? ? ? p. 
+  exact (set_label_to_mo_output (lts_outputs p)).
 Defined.
+Next Obligation.
+  intros ? ? ? ? ? ? p ? Hyp ;simpl in *.
+  unfold Inter_FW_obligation_1 in Hyp.
+  unfold set_label_to_mo_output in Hyp.
+  eapply elem_of_list_to_set in Hyp.
+  eapply elem_of_list_fmap in Hyp.
 
+  assert {y : A | ξ = label_to_output y ∧ y ∈ elements (lts_outputs p)} as wit.
+  eapply choice;eauto. intro.
+  destruct (decide (ξ = label_to_output x)).
+  + destruct (decide (x ∈ elements (lts_outputs p))).
+    ++ left; eauto.
+    ++ right. intros (Hyp1 & imp). contradiction.
+  + right. intros (imp & Hyp2). contradiction.
+  
+  + destruct wit as ( a & eq & mem ).
+    unfold label_to_output in eq; subst.
+    assert (a ∈ lts_outputs p) as mem'.
+    eapply elem_of_elements; eauto.
+    eapply lts_outputs_spec2 in mem'. 
+    eauto.
+Defined.
+Next Obligation.
+  intros ? ? ? ? ? ? q;simpl in *.
+  exact (set_label_to_mo_output (lts_outputs q)).
+Defined.
+Next Obligation.
+  intros ? ? ? ? ? ? q ? Hyp ;simpl in *.
+  unfold Inter_FW_obligation_1 in Hyp.
+  unfold set_label_to_mo_output in Hyp.
+  eapply elem_of_list_to_set in Hyp.
+  eapply elem_of_list_fmap in Hyp.
 
-#[global] Program Instance Inter_par
-  `{@Lts P A H} `{@Lts Q A H}: 
-    Prop_of_Inter P Q (ExtAct A) parallel_inter (* (@gLabel A H) gLts gLts *).
+  assert {x : A | ξ = label_to_output x ∧ x ∈ elements (lts_outputs q)} as wit.
+  eapply choice;eauto. intro.
+  destruct (decide (ξ = label_to_output x)).
+  + destruct (decide (x ∈ elements (lts_outputs q))).
+    ++ left; eauto.
+    ++ right. intros (Hyp1 & imp). contradiction.
+  + right. intros (imp & Hyp2). contradiction.
+  
+  + destruct wit as ( a & eq & mem ).
+    unfold label_to_output in eq; subst.
+    assert (a ∈ lts_outputs q) as mem'.
+    eapply elem_of_elements; eauto.
+    eapply lts_outputs_spec2 in mem'. 
+    eauto.
+Defined.
 Next Obligation.
-Admitted.
+  intros ? ? ? ? ? ? ? ? ? q ? q' ? ? inter;simpl in *.
+  unfold Inter_par_obligation_1. unfold Inter_par_obligation_3.
+  destruct α1 as [a (* input a *) | a (* output b *)].
+  + right. destruct inter as [case_1 | case_2].
+    ++ symmetry in case_1. eapply simplify_match_input in case_1 as eq; subst.
+       unfold set_label_to_mo_output.
+       eapply elem_of_list_to_set.
+       eapply elem_of_list_fmap. exists a. split; eauto. 
+       eapply elem_of_elements. eapply lts_outputs_spec1; eauto.
+    ++ eapply simplify_match_input in case_2 as eq; subst.
+       unfold set_label_to_mo_output.
+       eapply elem_of_list_to_set.
+       eapply elem_of_list_fmap. exists a. split; eauto. 
+       eapply elem_of_elements. eapply lts_outputs_spec1; eauto.
+  + left. 
+    eapply elem_of_list_to_set.
+    eapply elem_of_list_fmap. exists a. split; eauto. 
+    eapply elem_of_elements. eapply lts_outputs_spec1; eauto.
+Defined.
 Next Obligation.
-Admitted.
+  intros ? ? ? ? ? ? ξ p;simpl in *.
+  destruct ξ as [ a (* Input_case *) | a (* Ouput_case *)].
+  + exact empty. 
+  + exact {[ ActIn a ]}.
+Defined.
 Next Obligation.
-Admitted.
+  unfold Inter_FW_obligation_6.
+  unfold Inter_FW_obligation_3.
+  intros ? ? ? ? ? ? ? ? ? ? q mem l inter;simpl in *. 
+  eapply elem_of_list_to_set in mem.
+  eapply elem_of_list_fmap in mem.
+  destruct mem as ( a & eq & mem ); subst. simpl.
+  destruct inter as [case_1 | case_2]; unfold gLabel_nb_obligation_4 in *.
+  + eapply simplify_match_output in case_1. subst. set_solver.
+  + symmetry in case_2. eapply simplify_match_output in case_2. subst. set_solver.
+Defined.
 Next Obligation.
-Admitted.
+  intros ? ? ? ? ? ? ξ q;simpl in *.
+  destruct ξ as [ a (* Input_case *) | a (* Ouput_case *)].
+  + exact empty. 
+  + exact {[ ActIn a ]}.
+Defined.
 Next Obligation.
-Admitted.
-Next Obligation.
-Admitted.
-Next Obligation.
-Admitted.
-Next Obligation.
-Admitted.
-Next Obligation.
-Admitted.
+  unfold Inter_FW_obligation_6.
+  unfold Inter_FW_obligation_3.
+  intros ? ? ? ? ? ? ? ? ? ? q mem l inter;simpl in *. 
+  eapply elem_of_list_to_set in mem.
+  eapply elem_of_list_fmap in mem.
+  destruct mem as ( a & eq & mem ); subst. simpl.
+  destruct inter as [case_1 | case_2]; unfold gLabel_obligation_4 in *.
+  + symmetry in case_1. eapply simplify_match_output in case_1. subst. set_solver.
+  + eapply simplify_match_output in case_2. subst. set_solver.
+Defined. *)
 
-#[global] Program Instance Inter_FW_par
-  `{@Lts P A H} `{@Lts E A H}: Prop_of_Inter (P * mb A) E (ExtAct A) parallel_inter.
-Next Obligation.
-Admitted.
-Next Obligation.
-Admitted.
-Next Obligation.
-Admitted.
-Next Obligation.
-Admitted.
-Next Obligation.
-Admitted.
-Next Obligation.
-Admitted.
-Next Obligation.
-Admitted.
-Next Obligation.
-Admitted.
-Next Obligation.
-Admitted.
-
-Lemma com_only_with_non_blocking `{LtsP : Lts P A} (η : ExtAct A) η': 
-        dual η η' -> non_blocking η \/ non_blocking η'.
+Lemma com_only_with_output `{LtsP : Lts P A} (η : ExtAct A) η': 
+        dual η η' -> is_output η \/ is_output η'.
 Proof.
-Admitted.
+  intro duo. destruct η as [ a (* input *) | a (* input *) ].
+  + destruct duo as [case_1 | case_2].
+    ++ symmetry in case_1. eapply simplify_match_input in case_1 as eq; subst.
+       right. exists a. eauto.
+    ++ eapply simplify_match_input in case_2 as eq; subst.
+       right. exists a. eauto.
+  + destruct duo as [case_1 | case_2].
+    ++ symmetry in case_1. eapply simplify_match_output in case_1 as eq; subst.
+       left. exists a. eauto.
+    ++ eapply simplify_match_output in case_2 as eq; subst.
+       left. exists a. eauto.
+Qed.
 
-Lemma (p , m) 
+#[global] Program Instance VCCS_ggLts : gLts proc (ExtAct TypeOfActions) := ggLts gLabel_b.
 
+#[global] Program Instance VCCS_ggLtsEq : gLtsEq proc (ExtAct TypeOfActions) := 
+  ggLtsEq gLabel_b.
 
+#[global] Program Instance VCCS_gLtsOBA : gLtsOba proc (ExtAct TypeOfActions) := ggLtsOba_b.
+
+#[global] Program Instance VCCS_gLtsOBAFB : gLtsObaFB proc (ExtAct TypeOfActions) := ggLtsObaFB_b.
+
+#[global] Program Instance VCCS_gLtsOBAFW : gLtsObaFW proc (ExtAct TypeOfActions) := ggLtsObaFW_b.
+
+(* Definition all_action_are_blocking `{gLts P A} := forall μ, ¬ non_blocking μ. *)
+
+(* inutile *)
+(*
+Lemma FW_is_id_with_no_nb_actions
+  `{Lts P A} p α (m : A) : 
+  all_action_are_blocking ->
+  lts_refuses (p , m) α <-> lts_refuses p α.
+Proof.
+  split.
+  intro tr_in_fw.
+  destruct (decide (lts_refuses p α)) as [refuses | not_refuses].
+  + eauto.
+  + eapply lts_refuses_spec1 in not_refuses as (p' & l).
+    assert ({ q | @TransitionSystems.inter_step _ _ _ _ _ _ _ Inter_FW ((p ▷ m) : (P * TransitionSystems.mb (ExtAct ?A0))) α q }).
+    exists (p' , m). unfold TransitionSystems.lts_step. simpl in *.
+    unfold ggLts_obligation_1 in *.
+    eapply ParLeft.
+    exfalso. eapply lts_refuses_spec2.
+    eapply ParLeft in l.
+    assert (parallel_step (p , m) α (p' , m)). simpl in *.
+    eapply ParLeft. *)
+
+Lemma fw_does_all_input
+  `{@gLtsObaFW P (ExtAct A) (@gLabel_nb A L) LtsP LtsEqP LtsObaP} (p : P) μ:
+    ¬ output_are_non_blocking μ -> μ ∈ lts_acc_set_of p.
+Proof.
+  intro not_nb.
+  destruct μ.
+  + assert (output_are_non_blocking (ActOut a)) as nb.
+    exists a. eauto. assert (output_are_non_blocking (ActOut a)) as nb'. eauto.
+    destruct nb as (a' & eq); subst.
+    inversion eq. subst. assert (dual (ActIn a') (ActOut a')) as duo.
+    simpl. left. simpl. eauto.
+    destruct (TransitionSystems.lts_oba_fw_forward p (ActOut a') (ActIn a')) as (p' & Hyp).
+    simpl in *. unfold gLabel_nb_obligation_1 in Hyp.
+    eapply Hyp in nb';eauto. simpl in *.
+    eapply lts_refuses_spec2. exists p'.
+    destruct nb'. eauto.
+  + exfalso. assert (output_are_non_blocking (ActOut a)).
+    exists a; eauto. contradiction.
+Qed.
+
+Lemma retrieve_a_better_pre_order
+  `{@Lts P A L} `{@Lts Q A L} (p : P) (q : Q) :
+   (forall (p' : Q) μ, ¬ non_blocking μ -> μ ∈ lts_acc_set_of p') -> 
+    (lts_acc_set_of p ⊆ lts_acc_set_of q
+      <-> lts_outputs p ⊆ lts_outputs q).
+Proof.
+  intro fw_b_action.
+  split.
+  + intro inclusion. intro a. intro mem. eapply lts_outputs_spec2 in mem as (p2 & l).
+    assert ((ActOut a) ∈ lts_acc_set_of p) as mem.
+    eapply lts_refuses_spec2. simpl. eauto.
+    eapply inclusion in mem. eapply lts_refuses_spec1 in mem as (q' & l').
+    simpl in *. eapply lts_outputs_spec1 in l'. eauto.
+  + intro inclusion.
+    intros μ mem. destruct (decide (non_blocking μ)) as [nb | not_nb].
+    ++ inversion nb.
+    ++ eapply fw_b_action in not_nb; eauto.
+Qed.
+
+(* Lemma retrieve_a_better_pre_order_final
+  `{@gLtsObaFW P (ExtAct A) (@gLabel_nb A L) LtsP LtsEqP LtsObaP}
+  `{@gLtsObaFW Q (ExtAct A) (@gLabel_nb A L) LtsQ LtsEqQ LtsObaQ}
+    (p : P) (q : Q):
+    lts_acc_set_of p ⊆ lts_acc_set_of q
+      <-> lts_outputs p ⊆ lts_outputs q.
+Proof. *)
